Refactor names and more

theories/Examples/Tutorial/Parity.v
@@ -2,120 +2,148 @@ From stdpp Require Import prelude finite.
 From VLSM.Core Require Import VLSM PreloadedVLSM VLSMProjections Composition.
 From Coq Require Import FunctionalExtensionality.
 
-(** * Parity VLSM
+(** * The "multiplying" VLSMs
 
-  This module demonstrates some basic notions of the VLSM framework. We define
-  a (single) parity VLSM that stores a tuple and continually decrements one of the
-  tuple's elements while a constraint is checked at each step. The name originates
-  from the property of this VLSM to preserve the evenness of the tuple elements
-  difference ([parity_valid_states_same_parity]). The definitions and lemmas tap into
-  concepts such as valid and constrained traces, transitions, states, and messages.
+  This module demonstrates some basic notions of the VLSM framework.
+
+  We define a type of VLSM that stores an integer and continually decrements it
+  using input messages (also integers), while a constraint is checked at each step.
+  The definitions and lemmas tap into concepts such as valid and constrained
+  traces, transitions, states, and messages.
+
+  The "doubling" VLSM has 2 as the only initial message and outputs the doubles
+  of the messages it receives as input, which leads to constrained
+  messages being positive even numbers [doubling_constrained_messages] and,
+  combined with the only initial message being 2, the valid messages of the
+  doubling VLSM are powers of 2 [doubling_valid_messages_powers_of_2].
+
+  Similarly, the "tripling" VLSM has 3 as the only initial message and outputs
+  the triples of the messages it receives as input.
+  When putting them together, though, they become more than the sum of their
+  parts: for example, the free composition's valid messages are all integers
+  which can be decomposed as a product of powers of 2 and 3.
 *)
 
 #[local] Open Scope Z_scope.
 
-(** ** Definition of the Parity VLSM
+(** ** Definition of the multiplying VLSMs' common features
 
-  The Parity VLSM will only have one label, indicating a decrement.
-  For this reason, the [unit] type can be used.
+  The multiplying VLSMs have only one type of transition, decrementing their
+  state and multiplying their input message as an output.
+  For this reason, the [unit] type can be used as a label.
 *)
 
-Definition ParityLabel : Type := unit.
+Definition multiplying_label : Type := unit.
 
 (** The state will hold an integer. *)
 
-Definition ParityState : Type := Z.
+Definition multiplying_state : Type := Z.
 
 (** Messages are integers. *)
 
-Definition ParityMessage : Type := Z.
+Definition multiplying_message : Type := Z.
 
-(** A VLSM Type is defined using ParityState and ParityLabel. *)
+(** A VLSM Type is defined using [multiplying_state] and [multiplying_label]. *)
 
-Definition ParityType : VLSMType ParityMessage :=
+Definition multiplying_type : VLSMType multiplying_message :=
 {|
-  state := ParityState;
-  label := ParityLabel;
+  state := multiplying_state;
+  label := multiplying_label;
 |}.
 
 (**
-  The specifications for the initial state, transition
-  and guard predicate are as follows:
+  To improve readability, we explicitly define [multiply_label] as the value of
+  the unit type.
 *)
 
-Definition Parity_initial_state_prop (st : ParityState) : Prop :=
+Definition multiply_label : label multiplying_type := ().
+
+(** The initial states of multiplying VLSMs will be positive integers. *)
+
+Definition multiplying_initial_state_prop (st : multiplying_state) : Prop :=
   st >= 1.
-
-Definition Parity_transition
-  (l : ParityLabel) (st : ParityState) (om : option ParityMessage)
-  : ParityState * option ParityMessage :=
-  match om with
-  | Some j  => (st - j, Some (2 * j))
-  | None    => (st, None)
-  end.
-
-Definition Parity_valid
-  (l : ParityLabel) (st : ParityState) (om : option ParityMessage) : Prop :=
-  match om with
-  | Some msg => msg <= st /\ 2 <= msg
-  | None     => False
-  end.
 
 (**
   We must also provide a proof that the intial state type
   is inhabited as the set of initial states is non-empty.
 *)
 
-Definition Parity_initial_state_type : Type :=
-  {st : ParityState | Parity_initial_state_prop st}.
+Definition multiplying_initial_state_type : Type :=
+  {st : multiplying_state | multiplying_initial_state_prop st}.
 
-Program Definition Parity_initial_state :
-  Parity_initial_state_type := exist _ 1 _.
+Program Definition multiplying_initial_state :
+  multiplying_initial_state_type := exist _ 1 _.
 Next Obligation.
 Proof. done. Defined.
 
-#[export] Instance Parity_Inhabited_initial_state_type :
- Inhabited (Parity_initial_state_type) :=
-  populate (Parity_initial_state).
+#[export] Instance multiplying_initial_state_type_inhabited :
+ Inhabited (multiplying_initial_state_type) :=
+  populate (multiplying_initial_state).
+
+(**
+  The transition validity predicate is also common for all multiplying VLSMs:
+  themessage must exist, must be larger than 1 and not larger than the current state.
+*)
+
+Definition multiplying_valid
+  (l : multiplying_label) (st : multiplying_state) (om : option multiplying_message) : Prop :=
+  match om with
+  | Some msg => msg <= st /\ 2 <= msg
+  | None     => False
+  end.
+
+(** ** Definition of the doubling VLSM
+
+  The doubling VLSM is a multiplying VLSM whose initial message is 2 and which
+  outputs the double of the received input, while using it to decrement the
+  current state; the [multiplying_valid] constraint ensures that the valid/constraines
+  states don't become negative.
+
+  Not that, since the transition function must be total, it must also be defined
+  for the case in which no input is provided, although that case will be
+  filtered out by the transition validity predicate.
+*)
+
+Definition doubling_transition
+  (l : multiplying_label) (st : multiplying_state) (om : option multiplying_message)
+  : multiplying_state * option multiplying_message :=
+  match om with
+  | Some j  => (st - j, Some (2 * j))
+  | None    => (st, None)
+  end.
 
 (**
   An intermediate representation for the VLSM is required.
-  It uses the previously defined specifications.
+  It uses the previously defined specifications with the addition that it
+  states that 2 is the only initial message.
 *)
 
-Definition ParityMachine : VLSMMachine ParityType :=
+Definition doubling_machine : VLSMMachine multiplying_type :=
 {|
-  initial_state_prop := Parity_initial_state_prop;
-  initial_message_prop := fun (ms : ParityMessage) => ms = 2;
-  s0 := Parity_Inhabited_initial_state_type;
-  transition := fun l '(st, om) => Parity_transition l st om;
-  valid := fun l '(st, om) => Parity_valid l st om;
+  initial_state_prop := multiplying_initial_state_prop;
+  initial_message_prop := fun (ms : multiplying_message) => ms = 2;
+  s0 := multiplying_initial_state_type_inhabited;
+  transition := fun l '(st, om) => doubling_transition l st om;
+  valid := fun l '(st, om) => multiplying_valid l st om;
 |}.
 
-(** The definition of the Parity VLSM. *)
+(** The definition of the doubling VLSM. *)
 
-Definition ParityVLSM : VLSM ParityMessage :=
+Definition doubling_vlsm : VLSM multiplying_message :=
 {|
-  vtype := ParityType;
-  vmachine := ParityMachine;
+  vtype := multiplying_type;
+  vmachine := doubling_machine;
 |}.
 
-(**
-  To improve readability, we explicitly define [parity_label] as the value of
-  the unit type.
-*)
+(** *** Doubling VLSM Examples *)
 
-Definition parity_label : label ParityVLSM := ().
+(** **** Example of an arbitrary transition *)
 
-(** ** Parity VLSM Examples *)
-
-(** *** Example of an arbitrary transition *)
-
-Lemma parity_example_transition_1 `(X : VLSM ParityMessage) :
-  transition ParityVLSM parity_label (4, Some 10) = (-6, Some 20).
+Lemma doubling_example_transition_1 `(X : VLSM multiplying_message) :
+  transition doubling_vlsm multiply_label (4, Some 10) = (-6, Some 20).
 Proof. done. Qed.
 
-(** *** Example of a valid trace *)
+(** **** Example of a valid trace *)
 
 (** The initial state cannot be included to this definition, because, since there is no
     transition reaching this state, it cannot be expressed in the below manner
@@ -125,149 +153,149 @@ Proof. done. Qed.
     difference to the trace
 *)
 
-Definition parity_trace1_init : list (transition_item ParityVLSM) :=
-  [ Build_transition_item parity_label (Some 4)
+Definition doubling_trace1_init : list (transition_item doubling_vlsm) :=
+  [ Build_transition_item multiply_label (Some 4)
      4 (Some 8)
-  ; Build_transition_item parity_label (Some 2)
+  ; Build_transition_item multiply_label (Some 2)
      2 (Some 4) ].
 
-Definition parity_trace1_last_item : transition_item ParityVLSM :=
-  Build_transition_item parity_label (Some 2)
+Definition doubling_trace1_last_item : transition_item doubling_vlsm :=
+  Build_transition_item multiply_label (Some 2)
     0 (Some 4).
 
-Definition parity_trace1 : list (transition_item ParityVLSM) :=
-  parity_trace1_init ++ [parity_trace1_last_item].
+Definition doubling_trace1 : list (transition_item doubling_vlsm) :=
+  doubling_trace1_init ++ [doubling_trace1_last_item].
 
-Definition parity_trace1_first_state : ParityState := 8.
+Definition doubling_trace1_first_state : multiplying_state := 8.
 
-Definition parity_trace1_last_state : ParityState :=
-  destination parity_trace1_last_item.
+Definition doubling_trace1_last_state : multiplying_state :=
+  destination doubling_trace1_last_item.
 
 (** Defined trace is valid: *)
 
-Example parity_valid_message_prop_2 : valid_message_prop ParityVLSM 2.
+Example doubling_valid_message_prop_2 : valid_message_prop doubling_vlsm 2.
 Proof. by apply initial_message_is_valid. Qed.
 
-Example parity_can_emit_4 : can_emit ParityVLSM 4.
+Example doubling_can_emit_4 : can_emit doubling_vlsm 4.
 Proof.
-  exists (2, Some 2), parity_label, 0.
+  exists (2, Some 2), multiply_label, 0.
   repeat split; [| | by lia.. | by cbn; do 2 f_equal; lia].
-  - by apply initial_state_is_valid; cbn; unfold Parity_initial_state_prop; lia.
+  - by apply initial_state_is_valid; cbn; unfold multiplying_initial_state_prop; lia.
   - by app_valid_tran.
 Qed.
 
-Example parity_valid_message_prop_4 : valid_message_prop ParityVLSM 4.
+Example doubling_valid_message_prop_4 : valid_message_prop doubling_vlsm 4.
 Proof.
-  by apply (emitted_messages_are_valid ParityVLSM 4 parity_can_emit_4).
+  by apply (emitted_messages_are_valid doubling_vlsm 4 doubling_can_emit_4).
 Qed.
 
-Proposition parity_valid_transition_1 :
-  input_valid_transition ParityVLSM parity_label (8, Some 4) (4, Some 8).
+Proposition doubling_valid_transition_1 :
+  input_valid_transition doubling_vlsm multiply_label (8, Some 4) (4, Some 8).
 Proof.
   repeat split; [| | | by lia].
   - by apply initial_state_is_valid; cbn;
-      unfold Parity_initial_state_prop, parity_trace1_first_state; lia.
-  - by apply parity_valid_message_prop_4.
-  - by unfold parity_trace1_first_state; nia.
+      unfold multiplying_initial_state_prop, doubling_trace1_first_state; lia.
+  - by apply doubling_valid_message_prop_4.
+  - by unfold doubling_trace1_first_state; nia.
 Qed.
 
-Proposition parity_valid_transition_2 :
-  input_valid_transition ParityVLSM parity_label (4, Some 2) (2, Some 4).
+Proposition doubling_valid_transition_2 :
+  input_valid_transition doubling_vlsm multiply_label (4, Some 2) (2, Some 4).
 Proof.
   repeat split; [| | by lia..].
-  - by app_valid_tran; eapply parity_valid_transition_1; lia.
-  - by apply parity_valid_message_prop_2.
+  - by app_valid_tran; eapply doubling_valid_transition_1; lia.
+  - by apply doubling_valid_message_prop_2.
 Qed.
 
-Proposition parity_valid_transition_3 :
-  input_valid_transition ParityVLSM parity_label (2, Some 2) (0, Some 4).
+Proposition doubling_valid_transition_3 :
+  input_valid_transition doubling_vlsm multiply_label (2, Some 2) (0, Some 4).
 Proof.
   repeat split; [| | by lia..].
-  - by app_valid_tran; apply parity_valid_transition_2.
-  - by apply parity_valid_message_prop_2.
+  - by app_valid_tran; apply doubling_valid_transition_2.
+  - by apply doubling_valid_message_prop_2.
 Qed.
 
-Example parity_valid_trace1 :
-  finite_valid_trace_init_to ParityVLSM
-   parity_trace1_first_state parity_trace1_last_state parity_trace1.
+Example doubling_valid_trace1 :
+  finite_valid_trace_init_to doubling_vlsm
+   doubling_trace1_first_state doubling_trace1_last_state doubling_trace1.
 Proof.
   constructor; [| done].
   repeat apply finite_valid_trace_from_to_extend.
   - by eapply finite_valid_trace_from_to_empty,
-      input_valid_transition_destination, parity_valid_transition_3.
-  - by apply parity_valid_transition_3.
-  - by apply parity_valid_transition_2.
-  - by apply parity_valid_transition_1.
+      input_valid_transition_destination, doubling_valid_transition_3.
+  - by apply doubling_valid_transition_3.
+  - by apply doubling_valid_transition_2.
+  - by apply doubling_valid_transition_1.
 Qed.
 
-Example parity_valid_trace1_alt :
-  finite_valid_trace_init_to_alt ParityVLSM
-   parity_trace1_first_state parity_trace1_last_state parity_trace1.
+Example doubling_valid_trace1_alt :
+  finite_valid_trace_init_to_alt doubling_vlsm
+   doubling_trace1_first_state doubling_trace1_last_state doubling_trace1.
 Proof.
   constructor; [| done].
   by repeat apply mvt_extend; [.. | apply mvt_empty]; try done;
-    [apply parity_valid_message_prop_4 | apply parity_valid_message_prop_2 ..].
+    [apply doubling_valid_message_prop_4 | apply doubling_valid_message_prop_2 ..].
 Qed.
 
-(** *** Example of a constrained trace *)
+(** **** Example of a constrained trace *)
 
 (** Previously defined trace is obviously constrained, since it's valid *)
-Lemma parity_constrained_trace1 :
-  finite_constrained_trace_init_to_direct ParityVLSM
-   parity_trace1_first_state parity_trace1_last_state parity_trace1.
+Lemma doubling_constrained_trace1 :
+  finite_constrained_trace_init_to_direct doubling_vlsm
+   doubling_trace1_first_state doubling_trace1_last_state doubling_trace1.
 Proof.
   constructor; [| done].
   by repeat apply ct_extend; [.. | apply ct_empty].
 Qed.
 
-Definition parity_trace2_init : list (transition_item ParityVLSM) :=
-  [ Build_transition_item parity_label (Some 2) 5 (Some 4)
-  ; Build_transition_item parity_label (Some 2) 3 (Some 4) ].
+Definition doubling_trace2_init : list (transition_item doubling_vlsm) :=
+  [ Build_transition_item multiply_label (Some 2) 5 (Some 4)
+  ; Build_transition_item multiply_label (Some 2) 3 (Some 4) ].
 
-Definition parity_trace2_last_item : transition_item ParityVLSM :=
-  Build_transition_item parity_label (Some 3) 0 (Some 6).
+Definition doubling_trace2_last_item : transition_item doubling_vlsm :=
+  Build_transition_item multiply_label (Some 3) 0 (Some 6).
 
-Definition parity_trace2 : list (transition_item ParityVLSM) :=
-  parity_trace2_init ++ [parity_trace2_last_item].
+Definition doubling_trace2 : list (transition_item doubling_vlsm) :=
+  doubling_trace2_init ++ [doubling_trace2_last_item].
 
-Definition parity_trace2_init_first_state : ParityState := 7.
+Definition doubling_trace2_init_first_state : multiplying_state := 7.
 
-Definition parity_trace2_init_last_state : ParityState := 3.
+Definition doubling_trace2_init_last_state : multiplying_state := 3.
 
-Definition parity_trace2_last_state : ParityState :=
-  destination parity_trace2_last_item.
+Definition doubling_trace2_last_state : multiplying_state :=
+  destination doubling_trace2_last_item.
 
 (** The given trace is valid without the last transition. *)
 
-Proposition parity_valid_transition_1' :
-  input_valid_transition ParityVLSM parity_label
-   (parity_trace2_init_first_state, Some 2) (5, Some 4).
+Proposition doubling_valid_transition_1' :
+  input_valid_transition doubling_vlsm multiply_label
+   (doubling_trace2_init_first_state, Some 2) (5, Some 4).
 Proof. by app_valid_tran. Qed.
 
-Proposition parity_valid_transition_2' :
-  input_valid_transition ParityVLSM parity_label
+Proposition doubling_valid_transition_2' :
+  input_valid_transition doubling_vlsm multiply_label
    (5, Some 2) (3, Some 4).
-Proof. by app_valid_tran; apply parity_valid_transition_1'. Qed.
+Proof. by app_valid_tran; apply doubling_valid_transition_1'. Qed.
 
-Example parity_valid_trace2_init :
-  finite_valid_trace_init_to ParityVLSM
-   parity_trace2_init_first_state parity_trace2_init_last_state parity_trace2_init.
+Example doubling_valid_trace2_init :
+  finite_valid_trace_init_to doubling_vlsm
+   doubling_trace2_init_first_state doubling_trace2_init_last_state doubling_trace2_init.
 Proof.
   constructor; [| done].
   repeat apply finite_valid_trace_from_to_extend.
   - by eapply finite_valid_trace_from_to_empty,
-      input_valid_transition_destination, parity_valid_transition_2'.
-  - by apply parity_valid_transition_2'.
-  - by apply parity_valid_transition_1'.
+      input_valid_transition_destination, doubling_valid_transition_2'.
+  - by apply doubling_valid_transition_2'.
+  - by apply doubling_valid_transition_1'.
 Qed.
 
-Example parity_valid_trace2_init_alt :
-  finite_valid_trace_init_to_alt ParityVLSM
-   parity_trace2_init_first_state parity_trace2_init_last_state parity_trace2_init.
+Example doubling_valid_trace2_init_alt :
+  finite_valid_trace_init_to_alt doubling_vlsm
+   doubling_trace2_init_first_state doubling_trace2_init_last_state doubling_trace2_init.
 Proof.
   constructor; [| done].
   by repeat apply mvt_extend; [..| apply mvt_empty]; try done;
-    apply parity_valid_message_prop_2.
+    apply doubling_valid_message_prop_2.
 Qed.
 
 (**
@@ -275,81 +303,81 @@ Qed.
   without its last transition is constrained.
 *)
 
-Example parity_constrained_trace2_init :
-  finite_constrained_trace_init_to ParityVLSM
-   parity_trace2_init_first_state parity_trace2_init_last_state parity_trace2_init.
+Example doubling_constrained_trace2_init :
+  finite_constrained_trace_init_to doubling_vlsm
+   doubling_trace2_init_first_state doubling_trace2_init_last_state doubling_trace2_init.
 Proof.
   apply VLSM_incl_finite_valid_trace_init_to.
   - by apply vlsm_incl_pre_loaded.
-  - by apply parity_valid_trace2_init.
+  - by apply doubling_valid_trace2_init.
 Qed.
 
 (**
-  The trace is valid (in the preloaded Parity VLSM) without
+  The trace is valid (in the preloaded doubling VLSM) without
   its last element and appending it to the end also gives
-  a valid trace (in the preloaded Parity VLSM).
+  a valid trace (in the preloaded doubling VLSM).
   It follows that the full trace is constrained in
-  the original Parity VLSM.
+  the original doubling VLSM.
 *)
 
-Example parity_constrained_trace2 :
-  finite_constrained_trace_init_to ParityVLSM
-    parity_trace2_init_first_state parity_trace2_last_state parity_trace2.
+Example doubling_constrained_trace2 :
+  finite_constrained_trace_init_to doubling_vlsm
+    doubling_trace2_init_first_state doubling_trace2_last_state doubling_trace2.
 Proof.
-  destruct parity_constrained_trace2_init.
+  destruct doubling_constrained_trace2_init.
   split; [| done].
-  eapply (extend_right_finite_trace_from_to (pre_loaded_with_all_messages_vlsm ParityVLSM));
+  eapply (extend_right_finite_trace_from_to (pre_loaded_with_all_messages_vlsm doubling_vlsm));
     [done |].
   repeat split; [| | done..].
   - by eapply finite_valid_trace_from_to_last_pstate.
   - by apply any_message_is_valid_in_preloaded.
 Qed.
 
-(** *** Example of a valid transition
+(** **** Example of a valid transition
 
   The last transition of a valid trace is valid.
 *)
 
-Lemma parity_example_valid_transition :
-  input_valid_transition ParityVLSM parity_label
+Lemma doubling_example_valid_transition :
+  input_valid_transition doubling_vlsm multiply_label
    (2, Some 2) (0, Some 4).
 Proof.
-  apply (finite_valid_trace_from_to_last_transition ParityVLSM
-    parity_trace1_first_state parity_trace1_last_state
-    parity_trace1_init parity_trace1 parity_trace1_last_item); [| done].
-  by apply parity_valid_trace1.
+  apply (finite_valid_trace_from_to_last_transition doubling_vlsm
+    doubling_trace1_first_state doubling_trace1_last_state
+    doubling_trace1_init doubling_trace1 doubling_trace1_last_item); [| done].
+  by apply doubling_valid_trace1.
 Qed.
 
-(** *** Example of a constrained transition
+(** **** Example of a constrained transition
 
   The last transition of a constrained trace is constrained.
 *)
 
-Example parity_example_constrained_transition :
-  input_valid_transition (pre_loaded_with_all_messages_vlsm ParityVLSM) parity_label
+Example doubling_example_constrained_transition :
+  input_valid_transition (pre_loaded_with_all_messages_vlsm doubling_vlsm) multiply_label
    (3, Some 3) (0, Some 6).
 Proof.
   apply (finite_valid_trace_from_to_last_transition
-    (pre_loaded_with_all_messages_vlsm ParityVLSM)
-    parity_trace2_init_first_state parity_trace2_last_state parity_trace2_init
-    parity_trace2 parity_trace2_last_item); [| done].
-  by apply parity_constrained_trace2.
+    (pre_loaded_with_all_messages_vlsm doubling_vlsm)
+    doubling_trace2_init_first_state doubling_trace2_last_state doubling_trace2_init
+    doubling_trace2 doubling_trace2_last_item); [| done].
+  by apply doubling_constrained_trace2.
 Qed.
 
-(** ** Parity VLSM Properties *)
+(** *** Doubling VLSM Properties *)
 
-(** *** Inclusion into preloaded with all messages *)
+(** **** Inclusion into preloaded with all messages *)
 
-Lemma parity_valid_is_constrained :
-  VLSM_incl ParityVLSM (pre_loaded_with_all_messages_vlsm ParityVLSM).
+Lemma doubling_valid_is_constrained :
+  VLSM_incl doubling_vlsm (pre_loaded_with_all_messages_vlsm doubling_vlsm).
 Proof.
   by apply vlsm_incl_pre_loaded_with_all_messages_vlsm.
 Qed.
 
 (** *** Constrained messages are positive even integers *)
 
-Lemma parity_constrained_messages_left :
-  forall (m : ParityMessage), constrained_message_prop ParityVLSM m ->
+Lemma doubling_constrained_messages_left :
+  forall (m : multiplying_message), constrained_message_prop doubling_vlsm m ->
    Z.Even m /\ m >= 4.
 Proof.
   intros m ([s []] & [] & s' & (_ & _ & []) & Ht).
@@ -357,31 +385,31 @@ Proof.
   by split; [eexists | lia].
 Qed.
 
-Lemma parity_constrained_messages_right :
-  forall (m : ParityMessage), Z.Even m -> m >= 4 ->
-   constrained_message_prop ParityVLSM m.
+Lemma doubling_constrained_messages_right :
+  forall (m : multiplying_message), Z.Even m -> m >= 4 ->
+   constrained_message_prop doubling_vlsm m.
 Proof.
   intros m [n ->] Hmgt0.
-  exists (n, Some n), parity_label, 0.
+  exists (n, Some n), multiply_label, 0.
   repeat split; [| | by lia.. | by cbn; do 2 f_equal; lia].
   - apply initial_state_is_valid; cbn; red; lia.
   - by apply any_message_is_valid_in_preloaded.
 Qed.
 
-Lemma parity_constrained_messages :
-  forall (m : ParityMessage),
-   constrained_message_prop ParityVLSM m <-> (Z.Even m /\ m >= 4).
+Lemma doubling_constrained_messages :
+  forall (m : multiplying_message),
+   constrained_message_prop doubling_vlsm m <-> (Z.Even m /\ m >= 4).
 Proof.
   split.
-  - by apply parity_constrained_messages_left.
-  - by intros [? ?]; apply parity_constrained_messages_right.
+  - by apply doubling_constrained_messages_left.
+  - by intros [? ?]; apply doubling_constrained_messages_right.
 Qed.
 
 (** *** Constrained states property *)
 
-Lemma parity_constrained_states_right :
- forall (st : ParityState),
-  constrained_state_prop ParityVLSM st ->
+Lemma doubling_constrained_states_right :
+ forall (st : multiplying_state),
+  constrained_state_prop doubling_vlsm st ->
    st >= 0.
 Proof.
   induction 1 using valid_state_prop_ind.
@@ -390,32 +418,32 @@ Proof.
     by inversion Ht; subst; cbn in *; lia.
 Qed.
 
-Lemma parity_constrained_states_left :
-  forall (st : ParityState), st >= 0 ->
-    constrained_state_prop ParityVLSM st.
+Lemma doubling_constrained_states_left :
+  forall (st : multiplying_state), st >= 0 ->
+    constrained_state_prop doubling_vlsm st.
 Proof.
   intros st Hst.
   apply input_valid_transition_destination
-    with (l := parity_label) (s := st + 2) (om := Some 2) (om' := Some 4).
+    with (l := multiply_label) (s := st + 2) (om := Some 2) (om' := Some 4).
   repeat split; [| | by lia.. | by cbn; do 2 f_equal; lia].
   - apply initial_state_is_valid; cbn; red; lia.
   - by apply any_message_is_valid_in_preloaded.
 Qed.
 
-Lemma parity_constrained_states :
-  forall (st : ParityState),
-    constrained_state_prop ParityVLSM st <-> st >= 0.
+Lemma doubling_constrained_states :
+  forall (st : multiplying_state),
+    constrained_state_prop doubling_vlsm st <-> st >= 0.
 Proof.
   split.
-  - by apply parity_constrained_states_right.
-  - by apply parity_constrained_states_left.
+  - by apply doubling_constrained_states_right.
+  - by apply doubling_constrained_states_left.
 Qed.
 
 (** *** Powers of 2 greater or equal than 2 are valid messages *)
 
-Lemma parity_valid_messages_powers_of_2_right :
-  forall (m : ParityMessage),
-    valid_message_prop ParityVLSM m ->
+Lemma doubling_valid_messages_powers_of_2_right :
+  forall (m : multiplying_message),
+    valid_message_prop doubling_vlsm m ->
       exists p : Z, p >= 1 /\ m = 2 ^ p.
 Proof.
   intros m [s Hvsm].
@@ -434,9 +462,9 @@ Proof.
     by rewrite <- Z.pow_succ_r; [| lia].
 Qed.
 
-Lemma parity_valid_messages_powers_of_2_left :
+Lemma doubling_valid_messages_powers_of_2_left :
   forall (p : Z),
-    p >= 1 -> valid_message_prop ParityVLSM (2 ^ p).
+    p >= 1 -> valid_message_prop doubling_vlsm (2 ^ p).
 Proof.
   intros p Hp.
   assert (Hle : 0 <= p - 1) by lia.
@@ -447,7 +475,7 @@ Proof.
   apply natlike_ind; [by apply initial_message_is_valid; cbn; lia |].
   intros x Hxgt0 Hindh.
   apply emitted_messages_are_valid.
-  exists (2 ^ (x + 1), Some (2 ^ (x + 1))), parity_label, 0.
+  exists (2 ^ (x + 1), Some (2 ^ (x + 1))), multiply_label, 0.
   repeat split.
   - by apply initial_state_is_valid; cbn; red; lia.
   - by apply Hindh.
@@ -457,33 +485,33 @@ Proof.
   - by cbn; rewrite <- Z.pow_succ_r, Z.add_succ_l; [do 2 f_equal; lia | lia].
 Qed.
 
-Lemma parity_valid_messages_powers_of_2 : forall (m : ParityMessage),
-  valid_message_prop ParityVLSM m <->
+Lemma doubling_valid_messages_powers_of_2 : forall (m : multiplying_message),
+  valid_message_prop doubling_vlsm m <->
     exists p : Z, p >= 1 /\ m = 2 ^ p.
 Proof.
   split.
-  - by intros; apply parity_valid_messages_powers_of_2_right.
-  - by intros (p & Hpgt0 & [= ->]); apply parity_valid_messages_powers_of_2_left.
+  - by intros; apply doubling_valid_messages_powers_of_2_right.
+  - by intros (p & Hpgt0 & [= ->]); apply doubling_valid_messages_powers_of_2_left.
 Qed.
 
 (**
-  The constrained transition from [parity_example_constrained_transition]
+  The constrained transition from [doubling_example_constrained_transition]
   is not also valid.
 *)
-Example parity_example_constrained_transition_not_valid :
-  ~ input_valid_transition ParityVLSM parity_label
+Example doubling_example_constrained_transition_not_valid :
+  ~ input_valid_transition doubling_vlsm multiply_label
     (3, Some 3) (0, Some 6).
 Proof.
   intros [(_ & Hm & _) _].
-  apply parity_valid_messages_powers_of_2 in Hm as (p & Hp & Heq).
+  apply doubling_valid_messages_powers_of_2 in Hm as (p & Hp & Heq).
   rewrite <- (Z.succ_pred p) in Heq.
   by rewrite Z.pow_succ_r in Heq; lia.
 Qed.
 
-(** *** Valid states hold non-negative integers *)
+(** **** Valid states hold non-negative integers *)
 
-Lemma parity_valid_states_right (s : ParityState) :
-  valid_state_prop ParityVLSM s -> s >= 0.
+Lemma doubling_valid_states_right (s : multiplying_state) :
+  valid_state_prop doubling_vlsm s -> s >= 0.
 Proof.
   induction 1 using valid_state_prop_ind;
     [by cbn in Hs; red in Hs; lia |].
@@ -492,65 +520,98 @@ Proof.
   by destruct Hv; lia.
 Qed.
 
-Lemma parity_valid_states_left (s : ParityState) :
-  s >= 0 -> valid_state_prop ParityVLSM s.
+Lemma doubling_valid_states_left (s : multiplying_state) :
+  s >= 0 -> valid_state_prop doubling_vlsm s.
 Proof.
   intro.
   destruct (decide (s = 0)) as [-> |];
     [| by apply initial_state_is_valid; cbn; red; lia].
   apply input_valid_transition_destination
-      with (l := parity_label) (s := 2) (om := Some 2) (om' := Some 4).
+      with (l := multiply_label) (s := 2) (om := Some 2) (om' := Some 4).
   repeat split; cbn; [| | by lia..].
   - by apply initial_state_is_valid; cbn; red; lia.
   - by apply initial_message_is_valid.
 Qed.
 
-Lemma parity_valid_states :
-  forall (s : ParityState),
-  valid_state_prop ParityVLSM s <-> s >= 0.
+Lemma doubling_valid_states :
+  forall (s : multiplying_state),
+  valid_state_prop doubling_vlsm s <-> s >= 0.
 Proof.
   split.
-  - by apply parity_valid_states_right.
-  - by apply parity_valid_states_left.
+  - by apply doubling_valid_states_right.
+  - by apply doubling_valid_states_left.
 Qed.
 
+(** ** Definition of the tripling VLSM
 
-Section sec_radix23.
+  Similarly to the doubling VLSM, the tripling VLSM is a multiplying VLSM,
+  differing only by the fact that its initial message is 3 and that it
+  outputs the triple of the received input.
 
-Inductive index23 := two | three.
+  It can be shown that its constrained messages are multiples of three and that
+  its valid messages are powers of three, but the proofs will be similar as
+  those for the doubling VLSM so we will omit them. The development in module
+  [PrimesComposition] will make results for the doubling and tripling VLSM be
+  particular instances of more general results.
+*)
 
-
-#[local] Instance eq_dec_index23 : EqDecision index23.
-Proof. by intros x y; unfold Decision; decide equality. Qed.
-
-
-Definition Triple_transition
-  (l : ParityLabel) (st : ParityState) (om : option ParityMessage)
-  : ParityState * option ParityMessage :=
+Definition tripling_transition
+  (l : multiplying_label) (st : multiplying_state) (om : option multiplying_message)
+  : multiplying_state * option multiplying_message :=
   match om with
   | Some j  => (st - j, Some (3 * j))
   | None    => (st, None)
   end.
 
-Definition TripleMachine : VLSMMachine ParityType :=
+Definition tripling_machine : VLSMMachine multiplying_type :=
 {|
-  initial_state_prop := Parity_initial_state_prop;
-  initial_message_prop := fun (ms : ParityMessage) => ms = 3;
-  s0 := Parity_Inhabited_initial_state_type;
-  transition := fun l '(st, om) => Triple_transition l st om;
-  valid := fun l '(st, om) => Parity_valid l st om;
+  initial_state_prop := multiplying_initial_state_prop;
+  initial_message_prop := fun (ms : multiplying_message) => ms = 3;
+  s0 := multiplying_initial_state_type_inhabited;
+  transition := fun l '(st, om) => tripling_transition l st om;
+  valid := fun l '(st, om) => multiplying_valid l st om;
 |}.
 
-Definition TripleVLSM : VLSM ParityMessage := mk_vlsm TripleMachine.
+Definition tripling_vlsm : VLSM multiplying_message := mk_vlsm tripling_machine.
 
-Definition components_23 (i : index23) : VLSM ParityMessage :=
+(** ** Composition of doubling and tripling VLSMs *)
+
+Section sec_23_composition.
+
+(**
+  Since our notion of [composite_vlsm] is based on an indexed set of components,
+  we need to define a base index type
+*)
+
+Inductive index23 := two | three.
+
+#[local] Instance eq_dec_index23 : EqDecision index23.
+Proof. by intros x y; unfold Decision; decide equality. Qed.
+
+Definition components_23 (i : index23) : VLSM multiplying_message :=
   match i with
-  | two => ParityVLSM
-  | three => TripleVLSM
+  | two => doubling_vlsm
+  | three => tripling_vlsm
   end.
 
-Definition composite_state_23_sum (s : composite_state components_23) : Z :=
-  s two + s three.
+Definition state_23 (n m : Z) : composite_state components_23 :=
+  fun (i : index23) => match i with two => n | three => m end.
+
+Definition state00 := state_23 0 0.
+
+Definition state01 := state_23 0 1.
+
+Definition state10 := state_23 1 0.
+
+Definition state11 := state_23 1 1.
+
+Definition state12 := state_23 1 2.
+
+Definition state21 := state_23 2 1.
+
+Definition state22 := state_23 2 2.
+
+Definition state02 := state_23 0 2.
 
 Definition zproj (s : composite_state components_23) (i : index23) : Z :=
   match i with
@@ -558,25 +619,9 @@ Definition zproj (s : composite_state components_23) (i : index23) : Z :=
   | three => s three
   end.
 
-Definition constraint_23
-  (l : composite_label components_23)
-  (sm : composite_state components_23 * option ParityMessage) : Prop :=
-  let sm' := composite_transition components_23 l sm in
-  Z.Even (composite_state_23_sum sm.1 + composite_state_23_sum sm'.1).
+Definition free_composition_23 : VLSM multiplying_message :=
+  free_composite_vlsm components_23.
 
-Definition composition_23 : VLSM ParityMessage :=
-  composite_vlsm components_23 constraint_23.
-
-Definition final_state (s : composite_state components_23) :=
-  valid_state_prop composition_23 s /\
-  ~ exists
-    (l : composite_label components_23)
-    (om : option ParityMessage)
-    (som' : composite_state components_23 * option ParityMessage),
-      input_valid_transition composition_23 l (s, om) som'.
-
-Definition statenm (n m : Z) : composite_state components_23 :=
-  fun (i : index23) => match i with two => n | three => m end.
 
 Definition state00 := statenm 0 0.
 
@@ -590,28 +635,45 @@ Definition state12 := statenm 1 2.
 
 Definition state21 := statenm 2 1.
 
-Definition state22 := statenm 2 2.
+Definition composite_state_23_sum (s : composite_state components_23) : Z :=
+  s two + s three.
 
-Definition state02 := statenm 0 2.
+Definition parity_constraint_23
+  (l : composite_label components_23)
+  (sm : composite_state components_23 * option multiplying_message) : Prop :=
+  let sm' := composite_transition components_23 l sm in
+  Z.Even (composite_state_23_sum sm.1 + composite_state_23_sum sm'.1).
 
-Example valid_statenm_geq1 (n m : Z) (Hn : n >= 1) (Hm : m >= 1) :
-  valid_state_prop composition_23 (statenm n m).
+
+(**
+  Final states are valid state from which no further valid transition can be taken.
+*)
+Definition parity_23_final_state (s : composite_state components_23) :=
+  valid_state_prop parity_composition_23 s /\
+  ~ exists
+    (l : composite_label components_23)
+    (om : option multiplying_message)
+    (som' : composite_state components_23 * option multiplying_message),
+      input_valid_transition parity_composition_23 l (s, om) som'.
+
+Example valid_state_23_geq1 (n m : Z) (Hn : n >= 1) (Hm : m >= 1) :
+  valid_state_prop parity_composition_23 (state_23 n m).
 Proof.
   by apply initial_state_is_valid; intros []; cbn; red.
 Qed.
 
-Example valid_state11 : valid_state_prop composition_23 state11.
-Proof. by apply (valid_statenm_geq1 1 1); lia. Qed.
+Example valid_state11 : valid_state_prop parity_composition_23 state11.
+Proof. by apply (valid_state_23_geq1 1 1); lia. Qed.
 
-Example valid_state00 : valid_state_prop composition_23 state00.
+Example valid_state00 : valid_state_prop parity_composition_23 state00.
 Proof.
   apply input_valid_transition_destination
-    with (l := existT three parity_label) (s := state02) (om := Some 2) (om' := Some 6).
+    with (l := existT three multiply_label) (s := state02) (om := Some 2) (om' := Some 6).
   repeat split.
   - apply input_valid_transition_destination
-      with (l := existT two parity_label) (s := state22) (om := Some 2) (om' := Some 4).
+      with (l := existT two multiply_label) (s := state22) (om := Some 2) (om' := Some 4).
     repeat split.
-    + by apply valid_statenm_geq1.
+    + by apply valid_state_23_geq1.
     + apply initial_message_is_valid.
       exists two.
       assert (Hinit : initial_message_prop (components_23 two) 2) by done.
@@ -630,12 +692,12 @@ Proof.
   - by cbn; f_equal; extensionality i; destruct i; cbn; state_update_simpl; cbn.
 Qed.
 
-Example valid_state01 : valid_state_prop composition_23 state01.
+Example valid_state01 : valid_state_prop parity_composition_23 state01.
 Proof.
   apply input_valid_transition_destination
-    with (l := existT two parity_label) (s := state21) (om := Some 2) (om' := Some 4).
+    with (l := existT two multiply_label) (s := state21) (om := Some 2) (om' := Some 4).
   repeat split.
-  - by apply valid_statenm_geq1.
+  - by apply valid_state_23_geq1.
   - apply initial_message_is_valid.
     exists two.
     assert (Hinit : initial_message_prop (components_23 two) 2) by done.
@@ -646,12 +708,12 @@ Proof.
   - by cbn; f_equal; extensionality i; destruct i; cbn; state_update_simpl; cbn.
 Qed.
 
-Example valid_state10 : valid_state_prop composition_23 state10.
+Example valid_state10 : valid_state_prop parity_composition_23 state10.
 Proof.
   apply input_valid_transition_destination
-    with (l := existT three parity_label) (s := state12) (om := Some 2) (om' := Some 6).
+    with (l := existT three multiply_label) (s := state12) (om := Some 2) (om' := Some 6).
   repeat split.
-  - by apply valid_statenm_geq1.
+  - by apply valid_state_23_geq1.
   - apply initial_message_is_valid.
     exists two.
     assert (Hinit : initial_message_prop (components_23 two) 2) by done.
@@ -662,8 +724,8 @@ Proof.
   - by cbn; f_equal; extensionality i; destruct i; cbn; state_update_simpl; cbn.
 Qed.
 
-Lemma final_state_prop23_left (s : composite_state components_23) :
-  (s = state00 \/ s = state01 \/ s = state10 \/ s = state11) -> final_state s.
+Lemma parity_23_final_state_prop23_left (s : composite_state components_23) :
+  (s = state00 \/ s = state01 \/ s = state10 \/ s = state11) -> parity_23_final_state s.
 Proof.
   intros Hcases.
   split.
@@ -680,7 +742,7 @@ Proof.
 Qed.
 
 Lemma valid_state_23_pos :
-  forall (s : composite_state components_23), valid_state_prop composition_23 s ->
+  forall (s : composite_state components_23), valid_state_prop parity_composition_23 s ->
   forall (i : index23), zproj s i >= 0.
 Proof.
   intros s Hs; induction Hs using valid_state_prop_ind;
@@ -691,12 +753,19 @@ Proof.
     destruct i; cbn in *; state_update_simpl; lia.
 Qed.
 
-Lemma final_state_prop23_right (s : composite_state components_23) :
-  final_state s ->
-    (s two = 0 /\ s three = 0) \/ (s two = 0 /\ s three = 1) \/
-    (s two = 1 /\ s three = 0) \/ (s two = 1 /\ s three = 1).
+Lemma parity_23_final_state_prop23_right (s : composite_state components_23) :
+  parity_23_final_state s -> s = state00 \/ s = state01 \/ s = state10 \/ s = state11.
 Proof.
   intros [Hs Hfinal].
+  cut ((s two = 0 /\ s three = 0) \/ (s two = 0 /\ s three = 1) \/
+    (s two = 1 /\ s three = 0) \/ (s two = 1 /\ s three = 1)).
+  {
+    intros  [[] | [[] | [[] | []]]].
+    - by left; extensionality x; destruct x.
+    - by right; left; extensionality x; destruct x.
+    - by right; right; left; extensionality x; destruct x.
+    - by right; right; right; extensionality x; destruct x.
+  }
   destruct (decide ((s two = 0 /\ s three = 0) \/ (s two = 0 /\ s three = 1) \/
     (s two = 1 /\ s three = 0) \/ (s two = 1 /\ s three = 1))); [done |].
   contradict Hfinal.
@@ -730,5 +799,13 @@ Proof.
       by exists (s two + s three - 1); lia.
 Qed.
 
-End sec_radix23.
+Lemma parity_23_final_state_prop23_equiv (s : composite_state components_23) :
+  parity_23_final_state s <-> s = state00 \/ s = state01 \/ s = state10 \/ s = state11.
+Proof.
+  split.
+  - by apply parity_23_final_state_prop23_right.
+  - by apply parity_23_final_state_prop23_left.
+Qed.
+
+End sec_23_composition.
 
